Add dummy callback c definition and vst proof; Add empty int encoder spec

src/Lib/Callback/Dummy.v
@@ -1,23 +1,48 @@
-Require Import Core.Core Core.Tactics.
+Require Import Core.Core Core.Tactics Lib.VstLib Lib.Stdlib.
 Require Import VST.floyd.proofauto.
 Require Import VST.floyd.library.
-Require Import Clight.asn_application.
-Require Import Lib.VstLib Lib.Stdlib.
-Require Import Core.Notations.
+Require Import Clight.dummy.
 
 Instance CompSpecs : compspecs. make_compspecs prog. Defined.
+Definition Vprog : varspecs. mk_varspecs prog. Defined.
 
 Open Scope Z.
 
-Definition dummy_callback  : funspec :=
-    WITH  data_p : val, size : Z,
+Definition dummy_callback_spec  : funspec :=
+    WITH data_p : val, size : Z,
          key_p : val
     PRE [tptr tvoid, tuint, tptr tvoid]
-      PROP ()
+      PROP (0 <= size <= Int.max_unsigned)
       PARAMS (data_p; Vint (Int.repr size); key_p)
       GLOBALS ()
       SEP ()
     POST [tint]
       PROP ()
-      LOCAL (temp ret_temp Vzero)
+      LOCAL (temp ret_temp (if size =? 0 then (Vint (Int.repr (-1))) else Vzero))
       SEP (). 
+
+Definition dummy_callback : ident * funspec :=
+  DECLARE _dummy dummy_callback_spec.
+
+Definition Gprog := ltac:(with_library prog [dummy_callback]).
+
+Theorem bool_der_encode : semax_body Vprog Gprog f_dummy dummy_callback.
+Proof.
+  start_function.
+  forward_if (
+      PROP ( ) 
+      LOCAL (temp _t'1 (if size =? 0 
+                        then (Vint (Int.repr (-1))) 
+                        else Vzero);
+             temp _buffer data_p; temp _size (Vint (Int.repr size)); 
+             temp _application_specific_key key_p)  
+      SEP ()).
+  * (* if size = 0 *)
+    forward.
+    entailer!.
+  * (* if size <> 0 *)
+    forward.
+    entailer!.
+    break_if; [rewrite Z.eqb_eq in Heqb; congruence| reflexivity].
+  * forward.
+Qed.
