src/Lib/DWT/Vst.v
@@ -3,7 +3,7 @@ Require Import Core.Core Core.StructNormalizer VstLib DWT.Exec
 Require Import VST.floyd.proofauto.
 Require Import Clight.der_encoder.
 
-Definition new_cs := composites ++ (match find_cs 
+Definition composites := composites ++ (match find_cs 
                                             asn_application._overrun_encoder_key 
                                             asn_application.composites with
                       | Some r => [r]
@@ -12,38 +12,22 @@ Definition new_cs := composites ++ (match find_cs
 
 Definition Vprog : varspecs. 
 Proof.
-  set (cs := new_cs).
+  set (cs := composites).
   set (gd := global_definitions).
   set (pi := public_idents).
-  unfold new_cs in cs.
-  simpl (composites ++
-           match
-             find_cs
-               asn_application._overrun_encoder_key
-               asn_application.composites
-           with
-           | Some r => [r]
-           | None => []
-           end) in cs.
+  unfold composites in cs.
+  simpl in cs.
   set (prog := Clightdefs.mkprogram cs gd pi _main Logic.I).
   mk_varspecs prog. 
 Defined.
 
 Instance CompSpecs : compspecs. 
 Proof.
-  set (cs := new_cs).
+  set (cs := composites).
   set (gd := global_definitions).
   set (pi := public_idents).
-  unfold new_cs in cs.
-  simpl (composites ++
-           match
-             find_cs
-               asn_application._overrun_encoder_key
-               asn_application.composites
-           with
-           | Some r => [r]
-           | None => []
-           end) in cs.
+  unfold composites in cs.
+  simpl in cs.
   set (prog := Clightdefs.mkprogram cs gd pi _main Logic.I).
   make_compspecs prog.
 Defined.
@@ -52,13 +36,14 @@ Open Scope Z.
 
 Section Der_write_tags.
 
+Definition cbi := asn_application._overrun_encoder_cb.
+
 Definition der_write_tags_spec : ident * funspec :=
   DECLARE _der_write_tags
-  WITH (* pointer to type descriptor structure *) 
+  WITH gv : globals,
+       (* pointer to type descriptor structure *) 
        td_p : val, td : TYPE_descriptor,
        struct_len: Z, tag_mode : Z, last_tag_form : Z, tag : Z,
-       (* callback pointer *)
-       cb_p : val,
        (* callback argument pointer *)
        app_p : val,
        (* overrun_encoder_key fields *)
@@ -67,11 +52,10 @@ Definition der_write_tags_spec : ident * funspec :=
       tptr cb_type, tptr tvoid]
     PROP()
     PARAMS(td_p; Vint (Int.repr struct_len); Vint (Int.repr tag_mode);
-           Vint (Int.repr last_tag_form); Vint (Int.repr tag); cb_p; app_p)
-    GLOBALS()
+           Vint (Int.repr last_tag_form); Vint (Int.repr tag); (gv cbi); app_p)
+    GLOBALS(gv)
     SEP(data_at_ Tsh type_descriptor_s td_p ; 
-        data_at Tsh enc_key_s (mk_enc_key buf_p buf_size computed_size) app_p;
-        func_ptr' callback cb_p)
+        data_at Tsh enc_key_s (mk_enc_key buf_p buf_size computed_size) app_p)
     POST[tint]
       PROP()
       LOCAL(temp ret_temp 
@@ -97,7 +81,7 @@ Definition der_write_tags_spec : ident * funspec :=
                       (mk_enc_key buf_p buf_size (computed_size + size)) 
                       app_p));
           data_at_ Tsh type_descriptor_s td_p; 
-          func_ptr' callback cb_p).
+          func_ptr' callback (gv cbi)).
 
 Definition Gprog := ltac:(with_library prog [der_write_tags_spec]).
 
