src/Core/Tactics.v
@@ -1,3 +1,4 @@
+(*Require Import VST.floyd.proofauto.*)
 Require Import Core Int Notations.
 
 Ltac ints_to_Z :=
@@ -58,3 +59,49 @@ Ltac Zbool_to_Prop :=
         || rewrite Z.ltb_ge in * 
         || rewrite Z.ltb_lt in *).
 
+(*Tactic Notation "forward_if" constr(postL) constr(postP) constr(postS) :=
+  let l :=
+  lazymatch type of postL with
+  | localdef =>
+      match goal with
+      | |- semax _ (PROPx (?P) (LOCALx ?Q ?R)) _ _ =>
+          let Q' := remove_LOCAL2 constr:(cons postL nil) Q in
+          constr:(cons postL Q')
+      end
+  | list localdef =>
+      match goal with
+      | |- semax _ (PROPx (?P) (LOCALx ?Q ?R)) _ _ =>
+          let Q' := remove_LOCAL2 postL Q in
+          let Q'' := eval cbv iota zeta beta delta [app] in (postL ++ Q') in Q''
+      end
+  | _ => fail "First arg must be localdef or list localdef" 
+  end in 
+  let p :=
+  lazymatch type of postP with
+  | Prop =>
+      match goal with
+      | |- semax _ (PROPx (?P) ?Q) _ _ =>
+          constr:(cons postP P)
+      end
+  | list Prop =>
+      match goal with
+      | |- semax _ (PROPx (?P) ?Q) _ _ =>
+          let P' := eval cbv iota zeta beta delta [app] in (postP ++ P) in P'
+      end
+  | _ => fail "Second arg must be Prop or list Prop"
+  end in
+  lazymatch type of postS with
+  | mpred =>
+      match goal with
+      | |- semax _ (PROPx (?P) (LOCALx ?Q) SEPx (?R)) _ _ =>
+          (*let R' := modify_sep [postS] R in*)
+          forward_if_tac ((PROPx p) (LOCALx l) (SEPx R))
+      end
+  | list mpred =>
+      match goal with
+      | |- semax _ (PROPx (?P) (LOCALx ?Q) SEPx (?R)) _ _ =>
+          (*let R' := modify_sep postS R in*)
+          forward_if_tac ((PROPx p) (LOCALx l) (SEPx R))
+      end
+  | _ => fail "Third arg must be mpred or list mpred" 
+  end.*)
