src/Primitive/Int/VstDec.v
@@ -1,0 +1,16 @@
+(* Decoding fails : 
+   1) when calloc fails to allocate memory for the output structure sptr (FAIL) SEP spec
+   2) if ber_check_tags return FAIL (when?) or MORE (?) - executable spec
+   3) if not enough data according to length read (MORE) - executable spec
+   4) expected length doesn't fit into size (FAIL) ?
+
+        st->size = (int)length;
+	/* The following better be optimized away. */
+	if(sizeof(st->size) != sizeof(length)
+			&& (ber_tlv_len_t)st->size != length) {
+		st->size = 0;
+		ASN__DECODE_FAILED;
+	}
+
+   5) malloc buf allocation fails (FAIL) SEP spec
+ *)
